preparing a big theorem about the unfolding

thy/Call_Return_Unfolding.thy
@@ -1,5 +1,6 @@
 theory Call_Return_Unfolding
 imports Matching Ruleset_Update
+  "Common/RepeatStabilize"
 begin
 
 
@@ -714,30 +715,43 @@ lemma "process_call [''X'' \<mapsto> [Rule (Match b) Return, Rule (Match c) Acce
 
 
 
+text{*This is how a firewall processes a ruleset. 
+       It starts at a certain chain, usually INPUT, FORWARD, our OUTPUT (called @{term chain_name} in the lemma).
+       The firewall has a default action of accept or drop.
+      We can check @{const sanity_wf_ruleset} and the other assumptions at runtime.
+      Consequently, we can apply @{const repeat_stabilize} as often as we want.
+       *}
+
+theorem repeat_stabilize_process_call:
+    assumes "sanity_wf_ruleset \<Gamma>" and "chain_name \<in> set (map fst \<Gamma>)" and "default_action = Accept \<or> default_action = Drop"
+    shows "(map_of \<Gamma>),\<gamma>,p\<turnstile> \<langle>repeat_stabilize n (process_call (map_of \<Gamma>)) [Rule MatchAny (Call chain_name), Rule MatchAny default_action], s\<rangle> \<Rightarrow> t \<longleftrightarrow>
+           (map_of \<Gamma>),\<gamma>,p\<turnstile> \<langle>[Rule MatchAny (Call chain_name), Rule MatchAny default_action], s\<rangle> \<Rightarrow> t"
+proof -
+  have x: "sanity_wf_ruleset \<Gamma> \<Longrightarrow> rs \<in> ran (map_of \<Gamma>) \<Longrightarrow> wf_chain (map_of \<Gamma>) rs" for \<Gamma> and rs::"'a rule list"
+  apply(simp add: sanity_wf_ruleset_def wf_chain_def)
+  by fastforce
+
+  from assms(1) have 1: "\<forall>rsg \<in> ran (map_of \<Gamma>). wf_chain (map_of \<Gamma>) rsg"
+    apply(intro ballI)
+    apply(drule x, simp)
+    apply(simp)
+    done
+  let ?rs="[Rule MatchAny (Call chain_name), Rule MatchAny default_action]::'a rule list"
+  from assms(2,3) have 2: "wf_chain (map_of \<Gamma>) ?rs"
+    apply(simp add: wf_chain_def domD dom_map_of_conv_image_fst)
+    by blast
+
+  have "\<forall>rsg \<in> ran \<Gamma> \<union> {rs}. wf_chain \<Gamma> rsg \<Longrightarrow> 
+    \<Gamma>,\<gamma>,p\<turnstile> \<langle>repeat_stabilize n (process_call \<Gamma>) rs, s\<rangle> \<Rightarrow> t \<longleftrightarrow> \<Gamma>,\<gamma>,p\<turnstile> \<langle>rs, s\<rangle> \<Rightarrow> t" for \<Gamma> rs
+  by(simp add: repeat_stabilize_funpow unfolding_n_sound_complete)
+  moreover from 1 2 have "\<forall>rsg \<in> ran (map_of \<Gamma>) \<union> {?rs}. wf_chain (map_of \<Gamma>) rsg" by simp
+  ultimately show ?thesis by simp
+qed
 
 
 
-
-
-
-
-
-
-
-text{*repeat the application at most n times (param 1) until it stabilize*}
-fun repeat_stabilize :: "nat \<Rightarrow> ('a \<Rightarrow> 'a) \<Rightarrow> 'a \<Rightarrow> 'a" where
-  "repeat_stabilize 0 _ v = v" |
-  "repeat_stabilize (Suc n) f v = (let v_new = f v in if v = v_new then v else repeat_stabilize n f v_new)"
-
-lemma "repeat_stabilize n f v = (f^^n) v"
-  proof(induction n arbitrary: v)
-  case (Suc n)
-    have "f v = v \<Longrightarrow> (f^^n) v = v" by(induction n) simp_all
-    with Suc show ?case by(simp add: Let_def funpow_swap1)
-  qed(simp)
-
-
-
+(*
+(*TODO: maybe we need to move the whole thing to somewhere where we have the ternary semantics? to embeddings probably?*)
 (*can we replace the constant number of process_call calls with number of chain decls *)
 definition unfold_ruleset_CHAIN :: "string \<Rightarrow> action \<Rightarrow> 'a ruleset \<Rightarrow> 'a rule list" where
 "unfold_ruleset_CHAIN chain_name default_action rs = check_simple_ruleset
@@ -756,4 +770,6 @@ lemma "sanity_wf_ruleset \<Gamma> \<Longrightarrow>
     (map_of \<Gamma>),\<gamma>,p\<turnstile> \<langle>[Rule MatchAny (Call chain_name), Rule MatchAny default_action], s\<rangle> \<Rightarrow> t"
 nitpick
 oops
+*)
+
 end
