thy/Firewall_Common.thy
@@ -27,4 +27,47 @@ by (cases rs\<^sub>1) auto
 
 
 
+
+section{*Basic Algorithms*}
+text{*These algorithms should be valid for all firewall models. The corresponding proofs follow once the semantics are defined. *}
+
+
+text{*The actions Log and Empty do not modify the packet processing in any way. They can be removed.*}
+fun rm_LogEmpty :: "'a rule list \<Rightarrow> 'a rule list" where
+  "rm_LogEmpty [] = []" |
+  "rm_LogEmpty ((Rule _ Empty)#rs) = rm_LogEmpty rs" |
+  "rm_LogEmpty ((Rule _ Log)#rs) = rm_LogEmpty rs" |
+  "rm_LogEmpty (r#rs) = r # rm_LogEmpty rs"
+
+lemma rm_LogEmpty_filter: "rm_LogEmpty rs = filter (\<lambda>r. get_action r \<noteq> Log \<and> get_action r \<noteq> Empty) rs"
+ by(induction rs rule: rm_LogEmpty.induct) (simp_all)
+
+lemma rm_LogEmpty_seq: "rm_LogEmpty (rs1@rs2) = rm_LogEmpty rs1 @ rm_LogEmpty rs2"
+  by(simp add: rm_LogEmpty_filter)
+
+
+
+
+
+text{*Optimize away MatchAny matches*}
+fun opt_MatchAny_match_expr :: "'a match_expr \<Rightarrow> 'a match_expr" where
+  "opt_MatchAny_match_expr MatchAny = MatchAny" |
+  "opt_MatchAny_match_expr (Match a) = (Match a)" |
+  "opt_MatchAny_match_expr (MatchNot (MatchNot m)) = (opt_MatchAny_match_expr m)" |
+  "opt_MatchAny_match_expr (MatchNot m) = MatchNot (opt_MatchAny_match_expr m)" |
+  "opt_MatchAny_match_expr (MatchAnd MatchAny MatchAny) = MatchAny" |
+  "opt_MatchAny_match_expr (MatchAnd MatchAny m) = (opt_MatchAny_match_expr m)" |
+  (*note: remove recursive call to opt_MatchAny_match_expr to make it probably faster*)
+  "opt_MatchAny_match_expr (MatchAnd m MatchAny) = (opt_MatchAny_match_expr m)" |
+  "opt_MatchAny_match_expr (MatchAnd _ (MatchNot MatchAny)) = (MatchNot MatchAny)" |
+  "opt_MatchAny_match_expr (MatchAnd (MatchNot MatchAny) _) = (MatchNot MatchAny)" |
+  "opt_MatchAny_match_expr (MatchAnd m1 m2) = MatchAnd (opt_MatchAny_match_expr m1) (opt_MatchAny_match_expr m2)"
+(* without recursive call: need to apply multiple times until it stabelizes *)
+
+
+text{*It is still a good idea to apply @{const opt_MatchAny_match_expr} multiple times. Example:*}
+lemma "MatchNot (opt_MatchAny_match_expr (MatchAnd MatchAny (MatchNot MatchAny))) = MatchNot (MatchNot MatchAny)" by simp
+lemma "m = (MatchAnd (MatchAnd MatchAny MatchAny) (MatchAnd MatchAny MatchAny)) \<Longrightarrow> 
+  (opt_MatchAny_match_expr^^2) m \<noteq> opt_MatchAny_match_expr m" by(simp add: funpow_def)
+
 end
