thy/Semantics.thy
@@ -1126,33 +1126,7 @@ end
 
 
 
-
-
-text{*The actions Log and Empty do not modify the packet processing in any way. They can be removed.*}
-fun rm_LogEmpty :: "'a rule list \<Rightarrow> 'a rule list" where
-  "rm_LogEmpty [] = []" |
-  "rm_LogEmpty ((Rule _ Empty)#rs) = rm_LogEmpty rs" |
-  "rm_LogEmpty ((Rule _ Log)#rs) = rm_LogEmpty rs" |
-  "rm_LogEmpty (r#rs) = r # rm_LogEmpty rs"
-
-lemma rm_LogEmpty_filter: "rm_LogEmpty rs = filter (\<lambda>r. get_action r \<noteq> Log \<and> get_action r \<noteq> Empty) rs"
- by(induction rs rule: rm_LogEmpty.induct) (simp_all)
-
-
-lemma rm_LogEmpty_seq: "rm_LogEmpty (rs1@rs2) = rm_LogEmpty rs1 @ rm_LogEmpty rs2"
-  proof(induction rs1)
-  case Nil thus ?case by simp
-  next
-  case (Cons r rs) thus ?case
-    apply(cases r, rename_tac m a)
-    apply(simp)
-    apply(case_tac a)
-            apply(simp_all)
-    done
-  qed
-
-
-
+text{*Common Algorithms*}
 
 lemma iptables_bigstep_rm_LogEmpty: "\<Gamma>,\<gamma>,p\<turnstile> \<langle>rm_LogEmpty rs, s\<rangle> \<Rightarrow> t \<longleftrightarrow> \<Gamma>,\<gamma>,p\<turnstile> \<langle>rs, s\<rangle> \<Rightarrow> t"
 proof(induction rs arbitrary: s)
