thy/Semantics_Ternary/Matching_Ternary.thy
@@ -169,22 +169,6 @@ lemma matches_iff_apply_f: "ternary_ternary_eval (map_match_tac \<beta> p (f m))
 
 
 
-
-text{*Optimize away MatchAny matches*}
-fun opt_MatchAny_match_expr :: "'a match_expr \<Rightarrow> 'a match_expr" where
-  "opt_MatchAny_match_expr MatchAny = MatchAny" |
-  "opt_MatchAny_match_expr (Match a) = (Match a)" |
-  "opt_MatchAny_match_expr (MatchNot (MatchNot m)) = (opt_MatchAny_match_expr m)" |
-  "opt_MatchAny_match_expr (MatchNot m) = MatchNot (opt_MatchAny_match_expr m)" |
-  "opt_MatchAny_match_expr (MatchAnd MatchAny MatchAny) = MatchAny" |
-  "opt_MatchAny_match_expr (MatchAnd MatchAny m) = (opt_MatchAny_match_expr m)" |
-  (*note: remove recursive call to opt_MatchAny_match_expr to make it probably faster*)
-  "opt_MatchAny_match_expr (MatchAnd m MatchAny) = (opt_MatchAny_match_expr m)" |
-  "opt_MatchAny_match_expr (MatchAnd _ (MatchNot MatchAny)) = (MatchNot MatchAny)" |
-  "opt_MatchAny_match_expr (MatchAnd (MatchNot MatchAny) _) = (MatchNot MatchAny)" |
-  "opt_MatchAny_match_expr (MatchAnd m1 m2) = MatchAnd (opt_MatchAny_match_expr m1) (opt_MatchAny_match_expr m2)"
-(* without recursive call: need to apply multiple times until it stabelizes *)
-
 lemma opt_MatchAny_match_expr_correct: "matches \<gamma> (opt_MatchAny_match_expr m) = matches \<gamma> m"
   proof(case_tac \<gamma>, rename_tac \<beta> \<alpha>, clarify)
   fix \<beta> \<alpha>
@@ -200,10 +184,6 @@ lemma opt_MatchAny_match_expr_correct: "matches \<gamma> (opt_MatchAny_match_exp
     done
   qed
 
-text{*It is still a good idea to apply @{const opt_MatchAny_match_expr} multiple times. Example:*}
-lemma "MatchNot (opt_MatchAny_match_expr (MatchAnd MatchAny (MatchNot MatchAny))) = MatchNot (MatchNot MatchAny)" by simp
-lemma "m = (MatchAnd (MatchAnd MatchAny MatchAny) (MatchAnd MatchAny MatchAny)) \<Longrightarrow> 
-  (opt_MatchAny_match_expr^^2) m \<noteq> opt_MatchAny_match_expr m" by(simp add: funpow_def)
 
 
 text{*An @{typ "'p unknown_match_tac"} is wf if it behaves equal for @{const Reject} and @{const Drop} *}
