thy/Semantics_Ternary/Semantics_Ternary.thy
@@ -439,17 +439,6 @@ lemma approximating_bigstep_deterministic: "\<lbrakk> \<gamma>,p\<turnstile> \<l
 
 
 
-(*Okay, now we basically have a copy of those :( *)
-text{*The actions Log and Empty do not modify the packet processing in any way. They can be removed.*}
-fun rm_LogEmpty :: "'a rule list \<Rightarrow> 'a rule list" where
-  "rm_LogEmpty [] = []" |
-  "rm_LogEmpty ((Rule _ Empty)#rs) = rm_LogEmpty rs" |
-  "rm_LogEmpty ((Rule _ Log)#rs) = rm_LogEmpty rs" |
-  "rm_LogEmpty (r#rs) = r # rm_LogEmpty rs"
-
-lemma rm_LogEmpty_filter: "rm_LogEmpty rs = filter (\<lambda>r. get_action r \<noteq> Log \<and> get_action r \<noteq> Empty) rs"
- by(induction rs rule: rm_LogEmpty.induct) (simp_all)
-
 lemma rm_LogEmpty_fun_semantics: 
   "approximating_bigstep_fun \<gamma> p (rm_LogEmpty rs) s = approximating_bigstep_fun \<gamma> p rs s"
   proof(induction \<gamma> p rs s rule: approximating_bigstep_fun_induct)
@@ -460,30 +449,6 @@ lemma rm_LogEmpty_fun_semantics:
     case (Nomatch \<gamma> p m a rs) thus ?case by(cases a,simp_all)
     next
     case (Match \<gamma> p m a rs) thus ?case by(cases a,simp_all)
-  qed
-
-lemma rm_LogEmpty_fun_semantics: 
-  "approximating_bigstep_fun \<gamma> p (rm_LogEmpty rs) s = approximating_bigstep_fun \<gamma> p rs s"
-  proof(induction \<gamma> p rs s rule: approximating_bigstep_fun_induct)
-    case Empty thus ?case by(simp)
-    next
-    case Decision thus ?case by(simp add: Decision_approximating_bigstep_fun)
-    next
-    case (Nomatch \<gamma> p m a rs) thus ?case by(cases a,simp_all)
-    next
-    case (Match \<gamma> p m a rs) thus ?case by(cases a,simp_all)
-  qed
-
-lemma rm_LogEmpty_seq: "rm_LogEmpty (rs1@rs2) = rm_LogEmpty rs1 @ rm_LogEmpty rs2"
-  proof(induction rs1)
-  case Nil thus ?case by simp
-  next
-  case (Cons r rs) thus ?case
-    apply(cases r, rename_tac m a)
-    apply(simp)
-    apply(case_tac a)
-            apply(simp_all)
-    done
   qed
 
 
@@ -520,6 +485,7 @@ using rm_LogEmpty_seq apply metis
 done
 
 
+(*TODO: move?*)
 lemma rm_LogEmpty_simple_but_Reject: 
   "good_ruleset rs \<Longrightarrow> \<forall>r \<in> set (rm_LogEmpty rs). get_action r = Accept \<or> get_action r = Reject \<or> get_action r = Drop"
   proof(induction rs)
