thy/Common/RepeatStabilize.thy
@@ -1,0 +1,23 @@
+theory RepeatStabilize
+imports Main
+begin
+
+text{*Repeating something a number of times*}
+
+
+(*TODO: move to COMMON*)
+text{*repeat the application at most n times (param 1) until it stabilize*}
+fun repeat_stabilize :: "nat \<Rightarrow> ('a \<Rightarrow> 'a) \<Rightarrow> 'a \<Rightarrow> 'a" where
+  "repeat_stabilize 0 _ v = v" |
+  "repeat_stabilize (Suc n) f v = (let v_new = f v in if v = v_new then v else repeat_stabilize n f v_new)"
+
+lemma repeat_stabilize_funpow: "repeat_stabilize n f v = (f^^n) v"
+  proof(induction n arbitrary: v)
+  case (Suc n)
+    have "f v = v \<Longrightarrow> (f^^n) v = v" by(induction n) simp_all
+    with Suc show ?case by(simp add: Let_def funpow_swap1)
+  qed(simp)
+
+
+
+end
